src/QueryTactics.v
@@ -19,56 +19,56 @@ Require Import Ssromega.
      This tactic tries to solve statements that involve inequalities with 
      queries sizes.
    *)
-  Ltac leq_queries_size :=
+  Ltac leq_selections_size :=
     repeat match goal with
            | [|- context [ selection_size _]] => simp selection_size => /=
-           | [|- context[ (_ < queries_size_aux (_ :: _))%coq_nat] ] =>
-             rewrite {2}/queries_size_aux /= -/(queries_size_aux _); simp selection_size
+           | [|- context[ (_ < selections_size_aux (_ :: _))%coq_nat] ] =>
+             rewrite {2}/selections_size_aux /= -/(selections_size_aux _); simp selection_size
 
-           | [|- context [queries_size_aux [seq (_, σ) | σ <- ?σs] ] ] =>
-     rewrite [queries_size_aux [seq _ | _ <- _] ]/queries_size_aux /= -map_comp /funcomp map_id
+           | [|- context [selections_size_aux [seq (_, σ) | σ <- ?σs] ] ] =>
+     rewrite [selections_size_aux [seq _ | _ <- _] ]/selections_size_aux /= -map_comp /funcomp map_id
 
-           | [|- context [ queries_size_aux (_ ++ _) ]] => rewrite queries_size_aux_cat /=
-           | [|- context [ queries_size (_ ++ _)]] => rewrite queries_size_cat
+           | [|- context [ selections_size_aux (_ ++ _) ]] => rewrite selections_size_aux_cat /=
+           | [|- context [ selections_size (_ ++ _)]] => rewrite selections_size_cat
 
-           | [|- context [ queries_size (merge_selection_sets (find_queries_with_label ?s ?rname ?ty ?qs)) ]] =>
+           | [|- context [ selections_size (merge_selection_sets (find_queries_with_label ?s ?rname ?ty ?qs)) ]] =>
              let Hfleq := fresh in
              let Hmleq := fresh in
              have Hfleq := (found_queries_leq_size s rname ty qs);
              have Hmleq := (merged_selections_leq (find_queries_with_label s rname ty qs)); ssromega                         
 
-           | [|- context [queries_size_aux (merge_pairs_selection_sets ?s (find_valid_pairs_with_response_name ?s ?ts ?rname ?qs)) ]] =>
+           | [|- context [selections_size_aux (merge_pairs_selection_sets ?s (find_valid_pairs_with_response_name ?s ?ts ?rname ?qs)) ]] =>
              let Hfleq := fresh in
              let Hmleq := fresh in
              have Hfleq := (found_valid_pairs_leq_size s ts rname qs);
              have Hmleq := (merge_pair_selections_leq s (find_valid_pairs_with_response_name s ts rname qs)); ssromega
                                                                                                                           
-           | [|- context [ queries_size (merge_selection_sets (find_fields_with_response_name ?rname ?qs)) ]] =>
+           | [|- context [ selections_size (merge_selection_sets (find_fields_with_response_name ?rname ?qs)) ]] =>
               let Hfleq := fresh in
               let Hmleq := fresh in
               have Hfleq := (found_fields_leq_size rname qs);
               have Hmleq := (merged_selections_leq (find_fields_with_response_name rname qs)); ssromega
                                                                                                              
-            | [|- context [queries_size_aux (merge_pairs_selection_sets ?s (find_pairs_with_response_name ?rname ?qs)) ] ] =>
+            | [|- context [selections_size_aux (merge_pairs_selection_sets ?s (find_pairs_with_response_name ?rname ?qs)) ] ] =>
              let Hfleq := fresh in
              let Hmleq := fresh in
              have Hfleq := (found_pairs_with_response_name_leq rname qs);
              have Hmleq := (merge_pair_selections_leq s (find_pairs_with_response_name rname qs)); ssromega
                                                                                                
-           | [|- context [queries_size (merge_selection_sets ?qs)]] =>
+           | [|- context [selections_size (merge_selection_sets ?qs)]] =>
               let Hfleq := fresh in
               have Hfleq := (merged_selections_leq qs); ssromega                            
 
-           | [|- context [queries_size_aux (filter_pairs_with_response_name ?rname ?σs)] ] =>
+           | [|- context [selections_size_aux (filter_pairs_with_response_name ?rname ?σs)] ] =>
              let Hfleq := fresh in
              have Hfleq := (filter_pairs_with_response_name_leq rname σs); ssromega
                       
-           | [|- context [queries_size (filter_queries_with_label ?rname ?qs)]] =>
+           | [|- context [selections_size (filter_queries_with_label ?rname ?qs)]] =>
              let Hfleq := fresh in
              have Hfleq := (filter_queries_with_label_leq_size rname qs); ssromega
 
-           | [|- context [queries_size (filter_queries_with_label ?rname1 ?qs1) +
-                         queries_size (filter_queries_with_label ?rname2 ?qs2)]] =>
+           | [|- context [selections_size (filter_queries_with_label ?rname1 ?qs1) +
+                         selections_size (filter_queries_with_label ?rname2 ?qs2)]] =>
              let Hfleq1 := fresh in
              let Hfleq2 := fresh in
              have Hfleq1 := (filter_queries_with_label_leq_size rname1 qs1);
